new/code/github_com/goose_lang/primitive/disk.v
@@ -2,4 +2,28 @@
 From New.golang Require Import defn.
 
 Require Export New.trusted_code.github_com.goose_lang.primitive.disk.
+Import disk.
+From New Require Import disk_prelude.
+Module disk.
+Section code.
 
+
+Definition pkg_name' : go_string := "github.com/goose-lang/primitive/disk".
+
+Definition vars' : list (go_string * go_type) := [].
+
+Definition functions' : list (go_string * val) := [("Get"%go, Get); ("Read"%go, Read); ("Write"%go, Write); ("Size"%go, Size); ("Barrier"%go, Barrier)].
+
+Definition msets' : list (go_string * (list (go_string * val))) := [].
+
+Axiom _'init : val.
+
+Definition initialize' : val :=
+  rec: "initialize'" <> :=
+    globals.package_init pkg_name' vars' functions' msets' (λ: <>,
+      exception_do (do:  (_'init #());;;
+      do:  (_'init #()))
+      ).
+
+End code.
+End disk.
