new/generatedproof/go_etcd_io/raft/v3/raftpb.v
@@ -4,6 +4,285 @@ From New.golang Require Import theory.
 
 Axiom falso : False.
 
+Module Entry.
+Section def.
+Context `{ffi_syntax}.
+Record t := mk {
+  Term' : w64;
+  Index' : w64;
+  Type' : w32;
+  Data' : slice.t;
+}.
+End def.
+End Entry.
+
+
+Global Instance settable_Entry `{ffi_syntax}: Settable _ :=
+  settable! Entry.mk < Entry.Term'; Entry.Index'; Entry.Type'; Entry.Data' >.
+Global Instance into_val_Entry `{ffi_syntax} : IntoVal Entry.t.
+Admitted.
+
+Global Instance into_val_typed_Entry `{ffi_syntax} : IntoValTyped Entry.t raftpb.Entry :=
+{|
+  default_val := Entry.mk (default_val _) (default_val _) (default_val _) (default_val _);
+  to_val_has_go_type := ltac:(destruct falso);
+  default_val_eq_zero_val := ltac:(destruct falso);
+  to_val_inj := ltac:(destruct falso);
+  to_val_eqdec := ltac:(solve_decision);
+|}.
+Global Instance into_val_struct_field_Entry_Term `{ffi_syntax} : IntoValStructField "Term" raftpb.Entry Entry.Term'.
+Admitted.
+
+Global Instance into_val_struct_field_Entry_Index `{ffi_syntax} : IntoValStructField "Index" raftpb.Entry Entry.Index'.
+Admitted.
+
+Global Instance into_val_struct_field_Entry_Type `{ffi_syntax} : IntoValStructField "Type" raftpb.Entry Entry.Type'.
+Admitted.
+
+Global Instance into_val_struct_field_Entry_Data `{ffi_syntax} : IntoValStructField "Data" raftpb.Entry Entry.Data'.
+Admitted.
+
+Instance wp_struct_make_Entry `{ffi_semantics} `{!ffi_interp ffi} `{!heapGS Σ} Term' Index' Type' Data':
+  PureWp True
+    (struct.make raftpb.Entry (alist_val [
+      "Term" ::= #Term';
+      "Index" ::= #Index';
+      "Type" ::= #Type';
+      "Data" ::= #Data'
+    ]))%V
+    #(Entry.mk Term' Index' Type' Data').
+Admitted.
+
+Module ConfState.
+Section def.
+Context `{ffi_syntax}.
+Record t := mk {
+  Voters' : slice.t;
+  Learners' : slice.t;
+  VotersOutgoing' : slice.t;
+  LearnersNext' : slice.t;
+  AutoLeave' : bool;
+}.
+End def.
+End ConfState.
+
+
+Global Instance settable_ConfState `{ffi_syntax}: Settable _ :=
+  settable! ConfState.mk < ConfState.Voters'; ConfState.Learners'; ConfState.VotersOutgoing'; ConfState.LearnersNext'; ConfState.AutoLeave' >.
+Global Instance into_val_ConfState `{ffi_syntax} : IntoVal ConfState.t.
+Admitted.
+
+Global Instance into_val_typed_ConfState `{ffi_syntax} : IntoValTyped ConfState.t raftpb.ConfState :=
+{|
+  default_val := ConfState.mk (default_val _) (default_val _) (default_val _) (default_val _) (default_val _);
+  to_val_has_go_type := ltac:(destruct falso);
+  default_val_eq_zero_val := ltac:(destruct falso);
+  to_val_inj := ltac:(destruct falso);
+  to_val_eqdec := ltac:(solve_decision);
+|}.
+Global Instance into_val_struct_field_ConfState_Voters `{ffi_syntax} : IntoValStructField "Voters" raftpb.ConfState ConfState.Voters'.
+Admitted.
+
+Global Instance into_val_struct_field_ConfState_Learners `{ffi_syntax} : IntoValStructField "Learners" raftpb.ConfState ConfState.Learners'.
+Admitted.
+
+Global Instance into_val_struct_field_ConfState_VotersOutgoing `{ffi_syntax} : IntoValStructField "VotersOutgoing" raftpb.ConfState ConfState.VotersOutgoing'.
+Admitted.
+
+Global Instance into_val_struct_field_ConfState_LearnersNext `{ffi_syntax} : IntoValStructField "LearnersNext" raftpb.ConfState ConfState.LearnersNext'.
+Admitted.
+
+Global Instance into_val_struct_field_ConfState_AutoLeave `{ffi_syntax} : IntoValStructField "AutoLeave" raftpb.ConfState ConfState.AutoLeave'.
+Admitted.
+
+Instance wp_struct_make_ConfState `{ffi_semantics} `{!ffi_interp ffi} `{!heapGS Σ} Voters' Learners' VotersOutgoing' LearnersNext' AutoLeave':
+  PureWp True
+    (struct.make raftpb.ConfState (alist_val [
+      "Voters" ::= #Voters';
+      "Learners" ::= #Learners';
+      "VotersOutgoing" ::= #VotersOutgoing';
+      "LearnersNext" ::= #LearnersNext';
+      "AutoLeave" ::= #AutoLeave'
+    ]))%V
+    #(ConfState.mk Voters' Learners' VotersOutgoing' LearnersNext' AutoLeave').
+Admitted.
+
+Module SnapshotMetadata.
+Section def.
+Context `{ffi_syntax}.
+Record t := mk {
+  ConfState' : ConfState.t;
+  Index' : w64;
+  Term' : w64;
+}.
+End def.
+End SnapshotMetadata.
+
+
+Global Instance settable_SnapshotMetadata `{ffi_syntax}: Settable _ :=
+  settable! SnapshotMetadata.mk < SnapshotMetadata.ConfState'; SnapshotMetadata.Index'; SnapshotMetadata.Term' >.
+Global Instance into_val_SnapshotMetadata `{ffi_syntax} : IntoVal SnapshotMetadata.t.
+Admitted.
+
+Global Instance into_val_typed_SnapshotMetadata `{ffi_syntax} : IntoValTyped SnapshotMetadata.t raftpb.SnapshotMetadata :=
+{|
+  default_val := SnapshotMetadata.mk (default_val _) (default_val _) (default_val _);
+  to_val_has_go_type := ltac:(destruct falso);
+  default_val_eq_zero_val := ltac:(destruct falso);
+  to_val_inj := ltac:(destruct falso);
+  to_val_eqdec := ltac:(solve_decision);
+|}.
+Global Instance into_val_struct_field_SnapshotMetadata_ConfState `{ffi_syntax} : IntoValStructField "ConfState" raftpb.SnapshotMetadata SnapshotMetadata.ConfState'.
+Admitted.
+
+Global Instance into_val_struct_field_SnapshotMetadata_Index `{ffi_syntax} : IntoValStructField "Index" raftpb.SnapshotMetadata SnapshotMetadata.Index'.
+Admitted.
+
+Global Instance into_val_struct_field_SnapshotMetadata_Term `{ffi_syntax} : IntoValStructField "Term" raftpb.SnapshotMetadata SnapshotMetadata.Term'.
+Admitted.
+
+Instance wp_struct_make_SnapshotMetadata `{ffi_semantics} `{!ffi_interp ffi} `{!heapGS Σ} ConfState' Index' Term':
+  PureWp True
+    (struct.make raftpb.SnapshotMetadata (alist_val [
+      "ConfState" ::= #ConfState';
+      "Index" ::= #Index';
+      "Term" ::= #Term'
+    ]))%V
+    #(SnapshotMetadata.mk ConfState' Index' Term').
+Admitted.
+
+Module Snapshot.
+Section def.
+Context `{ffi_syntax}.
+Record t := mk {
+  Data' : slice.t;
+  Metadata' : SnapshotMetadata.t;
+}.
+End def.
+End Snapshot.
+
+
+Global Instance settable_Snapshot `{ffi_syntax}: Settable _ :=
+  settable! Snapshot.mk < Snapshot.Data'; Snapshot.Metadata' >.
+Global Instance into_val_Snapshot `{ffi_syntax} : IntoVal Snapshot.t.
+Admitted.
+
+Global Instance into_val_typed_Snapshot `{ffi_syntax} : IntoValTyped Snapshot.t raftpb.Snapshot :=
+{|
+  default_val := Snapshot.mk (default_val _) (default_val _);
+  to_val_has_go_type := ltac:(destruct falso);
+  default_val_eq_zero_val := ltac:(destruct falso);
+  to_val_inj := ltac:(destruct falso);
+  to_val_eqdec := ltac:(solve_decision);
+|}.
+Global Instance into_val_struct_field_Snapshot_Data `{ffi_syntax} : IntoValStructField "Data" raftpb.Snapshot Snapshot.Data'.
+Admitted.
+
+Global Instance into_val_struct_field_Snapshot_Metadata `{ffi_syntax} : IntoValStructField "Metadata" raftpb.Snapshot Snapshot.Metadata'.
+Admitted.
+
+Instance wp_struct_make_Snapshot `{ffi_semantics} `{!ffi_interp ffi} `{!heapGS Σ} Data' Metadata':
+  PureWp True
+    (struct.make raftpb.Snapshot (alist_val [
+      "Data" ::= #Data';
+      "Metadata" ::= #Metadata'
+    ]))%V
+    #(Snapshot.mk Data' Metadata').
+Admitted.
+
+Module HardState.
+Section def.
+Context `{ffi_syntax}.
+Record t := mk {
+  Term' : w64;
+  Vote' : w64;
+  Commit' : w64;
+}.
+End def.
+End HardState.
+
+
+Global Instance settable_HardState `{ffi_syntax}: Settable _ :=
+  settable! HardState.mk < HardState.Term'; HardState.Vote'; HardState.Commit' >.
+Global Instance into_val_HardState `{ffi_syntax} : IntoVal HardState.t.
+Admitted.
+
+Global Instance into_val_typed_HardState `{ffi_syntax} : IntoValTyped HardState.t raftpb.HardState :=
+{|
+  default_val := HardState.mk (default_val _) (default_val _) (default_val _);
+  to_val_has_go_type := ltac:(destruct falso);
+  default_val_eq_zero_val := ltac:(destruct falso);
+  to_val_inj := ltac:(destruct falso);
+  to_val_eqdec := ltac:(solve_decision);
+|}.
+Global Instance into_val_struct_field_HardState_Term `{ffi_syntax} : IntoValStructField "Term" raftpb.HardState HardState.Term'.
+Admitted.
+
+Global Instance into_val_struct_field_HardState_Vote `{ffi_syntax} : IntoValStructField "Vote" raftpb.HardState HardState.Vote'.
+Admitted.
+
+Global Instance into_val_struct_field_HardState_Commit `{ffi_syntax} : IntoValStructField "Commit" raftpb.HardState HardState.Commit'.
+Admitted.
+
+Instance wp_struct_make_HardState `{ffi_semantics} `{!ffi_interp ffi} `{!heapGS Σ} Term' Vote' Commit':
+  PureWp True
+    (struct.make raftpb.HardState (alist_val [
+      "Term" ::= #Term';
+      "Vote" ::= #Vote';
+      "Commit" ::= #Commit'
+    ]))%V
+    #(HardState.mk Term' Vote' Commit').
+Admitted.
+
+Module ConfChange.
+Section def.
+Context `{ffi_syntax}.
+Record t := mk {
+  Type' : w32;
+  NodeID' : w64;
+  Context' : slice.t;
+  ID' : w64;
+}.
+End def.
+End ConfChange.
+
+
+Global Instance settable_ConfChange `{ffi_syntax}: Settable _ :=
+  settable! ConfChange.mk < ConfChange.Type'; ConfChange.NodeID'; ConfChange.Context'; ConfChange.ID' >.
+Global Instance into_val_ConfChange `{ffi_syntax} : IntoVal ConfChange.t.
+Admitted.
+
+Global Instance into_val_typed_ConfChange `{ffi_syntax} : IntoValTyped ConfChange.t raftpb.ConfChange :=
+{|
+  default_val := ConfChange.mk (default_val _) (default_val _) (default_val _) (default_val _);
+  to_val_has_go_type := ltac:(destruct falso);
+  default_val_eq_zero_val := ltac:(destruct falso);
+  to_val_inj := ltac:(destruct falso);
+  to_val_eqdec := ltac:(solve_decision);
+|}.
+Global Instance into_val_struct_field_ConfChange_Type `{ffi_syntax} : IntoValStructField "Type" raftpb.ConfChange ConfChange.Type'.
+Admitted.
+
+Global Instance into_val_struct_field_ConfChange_NodeID `{ffi_syntax} : IntoValStructField "NodeID" raftpb.ConfChange ConfChange.NodeID'.
+Admitted.
+
+Global Instance into_val_struct_field_ConfChange_Context `{ffi_syntax} : IntoValStructField "Context" raftpb.ConfChange ConfChange.Context'.
+Admitted.
+
+Global Instance into_val_struct_field_ConfChange_ID `{ffi_syntax} : IntoValStructField "ID" raftpb.ConfChange ConfChange.ID'.
+Admitted.
+
+Instance wp_struct_make_ConfChange `{ffi_semantics} `{!ffi_interp ffi} `{!heapGS Σ} Type' NodeID' Context' ID':
+  PureWp True
+    (struct.make raftpb.ConfChange (alist_val [
+      "Type" ::= #Type';
+      "NodeID" ::= #NodeID';
+      "Context" ::= #Context';
+      "ID" ::= #ID'
+    ]))%V
+    #(ConfChange.mk Type' NodeID' Context' ID').
+Admitted.
+
 (* autogenerated by proofgen (names); do not modify *)
 Require Import New.code.go_etcd_io.raft.v3.raftpb.
 Require Export New.proof.proof_prelude.
